Move IntoVal and instances to separate file

src/goose_lang/lib/typed_map/typed_map.v
@@ -1,8 +1,5 @@
-From iris.proofmode Require Import coq_tactics reduction.
 From Perennial.goose_lang Require Import notation proofmode typing.
-(* TODO: slice and struct imports are only to provide IntoVal instances, maybe
-should factor out IntoVal *)
-From Perennial.goose_lang.lib Require Import typed_mem slice.slice struct.struct.
+From Perennial.goose_lang.lib Require Import typed_mem into_val.
 From Perennial.goose_lang.lib Require Import map.impl.
 From Perennial.goose_lang.lib Require map.map.
 Import uPred.
@@ -10,16 +7,6 @@ Import uPred.
 From iris_string_ident Require Import ltac2_string_ident.
 
 Set Default Proof Using "Type".
-
-Class IntoVal {ext: ext_op} V :=
-  { to_val: V -> val;
-    IntoVal_def: V;
-  }.
-
-Class IntoValForType {ext V} (H: @IntoVal ext V) {ext_ty: ext_types ext} (t:ty) :=
-    { def_is_zero: to_val IntoVal_def = zero_val t;
-      (* TODO: this isn't necessary, but it seems reasonable *)
-      to_val_ty: forall v, val_ty (to_val v) t; }.
 
 Module Map.
   Definition t V {ext} `{@IntoVal ext V} := gmap u64 V.
@@ -243,39 +230,3 @@ Arguments wp_NewMap {_ _ _ _ _ _ _} V {_} {t}.
 Arguments wp_MapGet {_ _ _ _ _ _} V {_} {_ _}.
 Arguments wp_MapInsert {_ _ _ _ _ _} V {_} {_ _}.
 Arguments wp_MapDelete {_ _ _ _ _ _} V {_} {_ _}.
-
-(** instances for IntoVal *)
-Section instances.
-  Context {ext: ext_op} {ext_ty: ext_types ext}.
-  Global Instance u64_IntoVal : IntoVal u64 :=
-    {| to_val := λ (x: u64), #x;
-       IntoVal_def := U64 0; |}.
-
-  Global Instance u64_IntoVal_uint64T : IntoValForType u64_IntoVal uint64T.
-  Proof.
-    constructor; auto.
-  Qed.
-
-  Global Instance loc_IntoVal : IntoVal loc :=
-    {| to_val := λ (l: loc), #l;
-       IntoVal_def := null;
-    |}.
-
-  Global Instance loc_IntoVal_ref t : IntoValForType loc_IntoVal (struct.ptrT t).
-  Proof.
-    constructor; auto.
-  Qed.
-
-  Global Instance slice_IntoVal : IntoVal Slice.t :=
-    {| to_val := slice_val;
-       IntoVal_def := Slice.nil;
-    |}.
-
-  Global Instance slice_IntoVal_ref t : IntoValForType slice_IntoVal (slice.T t).
-  Proof.
-    constructor; auto.
-    intros.
-    apply slice_val_ty.
-  Qed.
-
-End instances.
