src/goose_lang/lib/into_val.v
@@ -1,0 +1,48 @@
+From Perennial.goose_lang Require Import notation typing.
+From Perennial.goose_lang.lib Require Import typed_mem slice.slice struct.struct.
+
+Class IntoVal {ext: ext_op} V :=
+  { to_val: V -> val;
+    IntoVal_def: V;
+  }.
+
+Class IntoValForType {ext V} (H: @IntoVal ext V) {ext_ty: ext_types ext} (t:ty) :=
+    { def_is_zero: to_val IntoVal_def = zero_val t;
+      (* TODO: this isn't necessary, but it seems reasonable *)
+      to_val_ty: forall v, val_ty (to_val v) t; }.
+
+(** instances for IntoVal *)
+Section instances.
+  Context {ext: ext_op} {ext_ty: ext_types ext}.
+  Global Instance u64_IntoVal : IntoVal u64 :=
+    {| to_val := λ (x: u64), #x;
+       IntoVal_def := U64 0; |}.
+
+  Global Instance u64_IntoVal_uint64T : IntoValForType u64_IntoVal uint64T.
+  Proof.
+    constructor; auto.
+  Qed.
+
+  Global Instance loc_IntoVal : IntoVal loc :=
+    {| to_val := λ (l: loc), #l;
+       IntoVal_def := null;
+    |}.
+
+  Global Instance loc_IntoVal_ref t : IntoValForType loc_IntoVal (struct.ptrT t).
+  Proof.
+    constructor; auto.
+  Qed.
+
+  Global Instance slice_IntoVal : IntoVal Slice.t :=
+    {| to_val := slice_val;
+       IntoVal_def := Slice.nil;
+    |}.
+
+  Global Instance slice_IntoVal_ref t : IntoValForType slice_IntoVal (slice.T t).
+  Proof.
+    constructor; auto.
+    intros.
+    apply slice_val_ty.
+  Qed.
+
+End instances.
