src/program_proof/proof_prelude.v
@@ -6,7 +6,7 @@ From Perennial.Helpers Require Export ListLen BigOp Transitions iris.
 
 From Perennial.program_logic Require Export ghost_var.
 From Perennial.goose_lang Require Export proofmode wpc_proofmode array.
-From Perennial.goose_lang Require Export readonly.
+From Perennial.goose_lang Require Export readonly into_val.
 From Perennial.goose_lang.lib Require Export slice struct loop lock control.
 From Perennial.goose_lang.lib Require Export typed_map.typed_map.
 From Perennial.goose_lang Require Export ffi.disk.
